refactor: move ac proofs to Init.

src/Init/Data/AC.lean
@@ -3,10 +3,101 @@ Copyright (c) 2022 Microsoft Corporation. All rights reserved.
 Released under Apache 2.0 license as described in the file LICENSE.
 Authors: Dany Fabian
 -/
-import Lean.Meta.Tactic.AC.Basic
 
-namespace Lean.Meta.AC.Theory
-open Lean.Meta.AC
+prelude
+import Init.Classical
+import Init.Data.List
+
+namespace Lean.Data.AC
+inductive Expr
+  | var (x : Nat)
+  | op (lhs rhs : Expr)
+  deriving Inhabited, Repr, BEq
+
+structure Variable (op : α → α → α) where
+  value : α
+  neutral : Option $ IsNeutral op value
+
+structure Context (α : Type u) where
+  op : α → α → α
+  assoc : IsAssociative op
+  comm : Option $ IsCommutative op
+  idem : Option $ IsIdempotent op
+  vars : List (Variable op)
+  arbitrary : α
+
+class ContextInformation (α : Type u) where
+  isNeutral : α → Nat → Bool
+  isComm : α → Bool
+  isIdem : α → Bool
+
+class EvalInformation (α : Type u) (β : Type v) where
+  arbitrary : α → β
+  evalOp : α → β → β → β
+  evalVar : α → Nat → β
+
+def Context.var (ctx : Context α) (idx : Nat) : Variable ctx.op :=
+  ctx.vars.getD idx ⟨ctx.arbitrary, none⟩
+
+instance : ContextInformation (Context α) where
+  isNeutral ctx x := ctx.var x |>.neutral.isSome
+  isComm ctx := ctx.comm.isSome
+  isIdem ctx := ctx.idem.isSome
+
+instance : EvalInformation (Context α) α where
+  arbitrary ctx := ctx.arbitrary
+  evalOp ctx := ctx.op
+  evalVar ctx idx := ctx.var idx |>.value
+
+def eval (β : Type u) [EvalInformation α β] (ctx : α) : (ex : Expr) → β
+  | Expr.var idx => EvalInformation.evalVar ctx idx
+  | Expr.op l r => EvalInformation.evalOp ctx (eval β ctx l) (eval β ctx r)
+
+def Expr.toList : Expr → List Nat
+  | Expr.var idx => [idx]
+  | Expr.op l r => l.toList.append r.toList
+
+def evalList (β : Type u) [EvalInformation α β] (ctx : α) : List Nat → β
+  | [] => EvalInformation.arbitrary ctx
+  | [x] => EvalInformation.evalVar ctx x
+  | x :: xs => EvalInformation.evalOp ctx (EvalInformation.evalVar ctx x) (evalList β ctx xs)
+
+def insert (x : Nat) : List Nat → List Nat
+  | [] => [x]
+  | a :: as => if x < a then x :: a :: as else a :: insert x as
+
+def sort (xs : List Nat) : List Nat :=
+  let rec loop : List Nat → List Nat → List Nat
+    | acc, [] => acc
+    | acc, x :: xs => loop (insert x acc) xs
+  loop [] xs
+
+def mergeIdem (xs : List Nat) : List Nat :=
+  let rec loop : Nat → List Nat → List Nat
+    | curr, next :: rest =>
+      if curr = next then
+        loop curr rest
+      else
+        curr :: loop next rest
+    | curr, [] => [curr]
+
+  match xs with
+  | [] => []
+  | x :: xs => loop x xs
+
+def removeNeutrals [info : ContextInformation α] (ctx : α) : List Nat → List Nat
+  | [] => []
+  | [x] => [x]
+  | x :: xs =>
+    match info.isNeutral ctx x with
+    | true => removeNeutrals ctx xs
+    | false => x :: removeNeutrals ctx xs
+
+def norm [info : ContextInformation α] (ctx : α) (e : Expr) : List Nat :=
+  let xs := e.toList
+  let xs := removeNeutrals ctx xs
+  let xs := if info.isComm ctx then sort xs else xs
+  if info.isIdem ctx then mergeIdem xs else xs
 
 theorem List.two_step_induction
   {motive : List Nat → Sort u}
@@ -201,7 +292,10 @@ theorem Context.evalList_append
   : evalList α ctx (l.append r) = ctx.op (evalList α ctx l) (evalList α ctx r) := by
   induction l using List.two_step_induction with
   | empty => simp_all
-  | single x => simp [List.append, evalList, EvalInformation.evalOp]
+  | single x =>
+    cases r
+    . simp at h₂
+    . simp [List.append, evalList, EvalInformation.evalOp]
   | step x y ys ih => simp [List.append, evalList, EvalInformation.evalOp] at *; rw [ih]; simp [ctx.assoc.1]
 
 theorem Context.eval_toList (ctx : Context α) (e : Expr) : evalList α ctx e.toList = eval α ctx e := by
@@ -221,4 +315,4 @@ theorem Context.eq_of_norm (ctx : Context α) (a b : Expr) (h : norm ctx a = nor
   rw [eval_norm, eval_norm] at h
   assumption
 
-end Lean.Meta.AC.Theory
+end Lean.Data.AC
